@prefix dcterms: <http://purl.org/dc/terms/> .
@prefix owl: <http://www.w3.org/2002/07/owl#> .
@prefix pcdm:  <http://pcdm.org/models#> .
@prefix pcdmff: <http://pcdm.org/file-format-types#> .
@prefix pcdmworks: <http://pcdm.org/works#> .
@prefix rdf:  <http://www.w3.org/1999/02/22-rdf-syntax-ns#> .
@prefix rdfs: <http://www.w3.org/2000/01/rdf-schema#> .
@prefix utk: <https://ontology.lib.utk.edu/works#> .
@prefix xsd:   <http://www.w3.org/2001/XMLSchema#> .

utk:hasBehavior a rdf:Property ;
    rdfs:label "has behavior"@en ;
    rdfs:comment "Links a pcdm:Object to a specific IIIF presentation behavior."@en ;
    rdfs:range utk:Behavior ;
    rdfs:domain pcdm:Object ;
    rdfs:isDefinedBy utk: .

utk:hasType a rdf:Property ;
    rdfs:label "has type" ;
    rdfs:comment """
    Signifies that the subject of a triple is an instance of a class. This is closely related to rdf:type but exists
    since we can't reuse that property in Hyku.
    """@en ;
    rdfs:seeAlso rdf:type ;
    rdfs:isDefinedBy utk: .

utk:hasVideoThumbnail a rdf:Property ;
    rdfs:label "has video thumbnail"@en ;
    rdfs:comment "Links a Video file to a short clip that represents the resource via a temporal media fragment."@en ;
    rdfs:domain pcdmff:Video ;
    rdfs:range rdfs:Literal;
    rdfs:seeAlso <https://www.w3.org/TR/media-frags/#naming-time> ;
    rdfs:isDefinedBy utk: .

utk:hasWorkType a rdf:Property ;
    rdfs:label "has work type"@en ;
    rdfs:comment "Describes the work type of a pcdmworks:Work."@en ;
    rdfs:domain pcdmworks:Work ;
    rdfs:range utk:WorkType ;
    rdfs:isDefinedBy utk: .

utk:Behavior a rdfs:Class ;
    rdfs:label "Behavior"@en ;
    rdfs:comment "A feature that the publisher of IIIF content would prefer the client to use when presenting the resource."@en ;
    rdfs:seeAlso <https://iiif.io/api/presentation/3.0/#behavior> ;
    rdfs:isDefinedBy utk: .

utk:ImageWork a utk:WorkType ;
    rdfs:label "Image"@en ;
    rdfs:seeAlso <https://utk-future-dc-worktypes.readthedocs.io/en/latest/contents/2_image.html> ;
    rdfs:comment """
    Image works are works where the primary fileset is derived from an image file such as a TIF, JP2, or JPEG. The
    fileset is served by a IIIF Image Server and passed to a IIIF viewer on the Work page by a IIIF Presentation 3
    manifest.
    """@en .

utk:NonPaged a utk:Behavior ;
    rdfs:label "non-paged"@en ;
    rdfs:seeAlso <https://iiif.io/api/presentation/3.0/#behavior> ;
    rdfs:comment """
    Valid only on Canvases, where the Canvas has at least height and width dimensions. Canvases that have this behavior
    must not be presented in a page turning interface, and must be skipped over when determining the page order. This
    behavior must be ignored if the current Manifest does not have the behavior value paged. Disjoint with paged and
    facing-pages.
    """@en .

utk:Paged a utk:Behavior ;
    rdfs:label "paged"@en ;
    rdfs:seeAlso <https://iiif.io/api/presentation/3.0/#behavior> ;
    rdfs:comment """
    Valid on Collections, Manifests and Ranges, which include Canvases that have at least height and width dimensions.
    Canvases included in resources that have this behavior represent views that should be presented in a page-turning
    interface if one is available. The first canvas is a single view (the first recto) and thus the second canvas likely
    represents the back of the object in the first canvas. If this is not the case, see the behavior value non-paged.
    Disjoint with unordered, individuals, continuous, facing-pages and non-paged.
    """@en .

utk:Unordered a utk:Behavior ;
    rdfs:label "unordered"@en ;
    rdfs:seeAlso <https://iiif.io/api/presentation/3.0/#behavior> ;
    rdfs:comment """
    Valid on Collections, Manifests and Ranges. The Canvases included in resources that have this behavior have no
    inherent order, and user interfaces should avoid implying an order to the user. Disjoint with individuals,
    continuous, and paged.
    """@en .

utk:WorkType a pcdmworks:Work ;
    rdfs:label "Work Type"@en ;
    rdfs:comment """
    Valid on pcdm:Works, a Work Type describes the data model and user expectations associated with a work.
    """@en .

utk: dcterms:modified "2022-07-02"^^xsd:date ;
    dcterms:publisher <http://www.lib.utk.edu/> ;
    dcterms:title "University of Tennessee Digital Initiatives Files and Works Ontology"@en ;
    rdfs:comment """
    Ontology for the the University of Tennessee Libraries to state relationships about works and the files they consist
    of.  This ontology does not intend to supersede more established ontologies but instead exists to state relationships
    when established properties cannot be identified.."""@en ;
    rdfs:seeAlso <https://github.com/utkdigitalinitiatives/utk_ontology/> ;
    owl:versionInfo "2022/07/05" .
