@prefix dcterms: <http://purl.org/dc/terms/> .
@prefix owl: <http://www.w3.org/2002/07/owl#> .
@prefix pcdm:  <http://pcdm.org/models#> .
@prefix pcdmff: <http://pcdm.org/file-format-types#> .
@prefix pcdmworks: <http://pcdm.org/works#> .
@prefix rdf:  <http://www.w3.org/1999/02/22-rdf-syntax-ns#> .
@prefix rdfs: <http://www.w3.org/2000/01/rdf-schema#> .
@prefix utk: <https://ontology.lib.utk.edu/works#> .
@prefix xsd:   <http://www.w3.org/2001/XMLSchema#> .

utk:hasBehavior a rdf:Property ;
    rdfs:label "has behavior"@en ;
    rdfs:comment "Links a pcdm:Object to a specific IIIF presentation behavior."@en ;
    rdfs:range utk:Behavior ;
    rdfs:domain pcdm:Object ;
    rdfs:isDefinedBy utk: .

utk:hasType a rdf:Property ;
    rdfs:label "has type" ;
    rdfs:comment """
    Signifies that the subject of a triple is an instance of a class. This is closely related to rdf:type but exists
    since we can't reuse that property in Hyku.
    """@en ;
    rdfs:seeAlso rdf:type ;
    rdfs:isDefinedBy utk: .

utk:hasVideoThumbnail a rdf:Property ;
    rdfs:label "has video thumbnail"@en ;
    rdfs:comment "Links a Video file to a short clip that represents the resource via a temporal media fragment."@en ;
    rdfs:domain pcdmff:Video ;
    rdfs:range rdfs:Literal;
    rdfs:seeAlso <https://www.w3.org/TR/media-frags/#naming-time> ;
    rdfs:isDefinedBy utk: .

utk:hasWorkType a rdf:Property ;
    rdfs:label "has work type"@en ;
    rdfs:comment "Describes the work type of a pcdmworks:Work."@en ;
    rdfs:domain pcdmworks:Work ;
    rdfs:range utk:WorkType ;
    rdfs:isDefinedBy utk: .

utk:AudioWork a utk:WorkType ;
    rdfs:label "Audio"@en ;
    rdfs:seeAlso <https://utk-future-dc-worktypes.readthedocs.io/en/latest/contents/4_audio.html> ;
    rdfs:comment """
    Audio works are works where the primary fileset(s) are derived from one or more audio files. The fileset(s) should
    be served to a IIIF viewer on the Work page by a IIIF Presentation 3 manifest. While there may be multiple filesets,
    there should only be one canvas with multiple annotations.
    """@en .

utk:Behavior a rdfs:Class ;
    rdfs:label "Behavior"@en ;
    rdfs:comment "A feature that the publisher of IIIF content would prefer the client to use when presenting the resource."@en ;
    rdfs:seeAlso <https://iiif.io/api/presentation/3.0/#behavior> ;
    rdfs:isDefinedBy utk: .

utk:BookWork a utk:WorkType ;
    rdfs:label "Book"@en ;
    rdfs:seeAlso <https://utk-future-dc-worktypes.readthedocs.io/en/latest/contents/6_books_and_pages.html> ;
    rdfs:comment """
    Book works are works that are made up of 1 to many pages that are intended to be served in a IIIF viewer as a paged
    object.
    """@en .

utk:CompoundObjectWork a utk:WorkType ;
    rdfs:label "Compound Object"@en ;
    rdfs:seeAlso <https://utk-future-dc-worktypes.readthedocs.io/en/latest/contents/7_compound_objects.html> ;
    rdfs:comment """
    Compound object works are works that are made up of 2 or more works. These works can be a combination of images,
    audio, video, and/or books. Compound objects are special in that the works the objects consist of are significant
    enough that they are able to stand alone in the wild in a system like the Digital Public Library of America. These
    sub parts have significant metadata which should lead to their inclusion in OAI-PMH. For the sake of user
    experience, parts of compound objects may not be displayed as stand alone objects in the same collection of a parent
    compound object.
    """@en .

utk:GenericWork a utk:WorkType ;
    rdfs:label "Generic Work"@en ;
    rdfs:seeAlso <https://utk-future-dc-worktypes.readthedocs.io/en/latest/contents/1_generic.html> ;
    rdfs:comment """
    Generic works are works where the primary fileset(s) are binary with no complex expectations for user experience or
    viewer in the browser. Instead, the primary purpose of this work type is to preserve and make available to users
    binary file types such as WARCs or born digital objects.
    """@en .

utk:ImageWork a utk:WorkType ;
    rdfs:label "Image"@en ;
    rdfs:seeAlso <https://utk-future-dc-worktypes.readthedocs.io/en/latest/contents/2_image.html> ;
    rdfs:comment """
    Image works are works where the primary fileset is derived from an image file such as a TIF, JP2, or JPEG. The
    fileset is served by a IIIF Image Server and passed to a IIIF viewer on the Work page by a IIIF Presentation 3
    manifest.
    """@en .

utk:NewspaperWork a utk:WorkType ;
    rdfs:label "Newspaper"@en ;
    rdfs:seeAlso <https://utk-future-dc-worktypes.readthedocs.io/en/latest/contents/8_newspapers.html> ;
    rdfs:comment """
    Newspaper works are perhaps our most complex worktype. Unlike books and compound objects, newspapers have a
    hierarchical structure that starts with a title, breaks down into volumes, and further down into issues. The date
    of publication and access to OCR data via METS / ALTO are critical to the viewing experience.
    """@en .

utk:NonPaged a utk:Behavior ;
    rdfs:label "non-paged"@en ;
    rdfs:seeAlso <https://iiif.io/api/presentation/3.0/#behavior> ;
    rdfs:comment """
    Valid only on Canvases, where the Canvas has at least height and width dimensions. Canvases that have this behavior
    must not be presented in a page turning interface, and must be skipped over when determining the page order. This
    behavior must be ignored if the current Manifest does not have the behavior value paged. Disjoint with paged and
    facing-pages.
    """@en .

utk:Paged a utk:Behavior ;
    rdfs:label "paged"@en ;
    rdfs:seeAlso <https://iiif.io/api/presentation/3.0/#behavior> ;
    rdfs:comment """
    Valid on Collections, Manifests and Ranges, which include Canvases that have at least height and width dimensions.
    Canvases included in resources that have this behavior represent views that should be presented in a page-turning
    interface if one is available. The first canvas is a single view (the first recto) and thus the second canvas likely
    represents the back of the object in the first canvas. If this is not the case, see the behavior value non-paged.
    Disjoint with unordered, individuals, continuous, facing-pages and non-paged.
    """@en .

utk:PDFWork a utk:WorkType ;
    rdfs:label "PDF"@en ;
    rdfs:seeAlso <https://utk-future-dc-worktypes.readthedocs.io/en/latest/contents/5_pdf.html> ;
    rdfs:comment """
    PDF works are works where the primary fileset(s) are PDFs. PDFs should minimally display something that allows the
    item to be opened in a new tab or with the PDF.js viewer.
    """@en .

utk:Unordered a utk:Behavior ;
    rdfs:label "unordered"@en ;
    rdfs:seeAlso <https://iiif.io/api/presentation/3.0/#behavior> ;
    rdfs:comment """
    Valid on Collections, Manifests and Ranges. The Canvases included in resources that have this behavior have no
    inherent order, and user interfaces should avoid implying an order to the user. Disjoint with individuals,
    continuous, and paged.
    """@en .

utk:VideoWork a utk:WorkType ;
    rdfs:label "Video"@en ;
    rdfs:seeAlso <https://utk-future-dc-worktypes.readthedocs.io/en/latest/contents/3_video.html> ;
    rdfs:comment """
    Video works are works where the primary fileset is derived from a video file. The file should be served to a IIIF
    viewer on the Work page by a IIIF Presentation 3 manifest.
    """@en .

utk:WorkType a pcdmworks:Work ;
    rdfs:label "Work Type"@en ;
    rdfs:comment """
    Valid on pcdm:Works, a Work Type describes the data model and user expectations associated with a work.
    """@en .

utk: dcterms:modified "2022-12-12"^^xsd:date ;
    dcterms:publisher <http://www.lib.utk.edu/> ;
    dcterms:title "University of Tennessee Digital Initiatives Files and Works Ontology"@en ;
    rdfs:comment """
    Ontology for the University of Tennessee Libraries to state relationships about works and the files they consist of.
    This ontology does not intend to supersede more established ontologies but instead exists to state relationships
    when established properties cannot be identified."""@en ;
    rdfs:seeAlso <https://github.com/utkdigitalinitiatives/utk_ontology/> ;
    owl:versionInfo "2022-12-12" .
